Finalise the module for trace swaps

src/TraceSwap.v
@@ -5,167 +5,350 @@ Import ListNotations.
 
 Open Scope list_scope.
 
-Section TraceSwapConstructive.
-
-Variable A : Type.
-
-Record t_constructive_gen l1 l2 rest x y (t t' : trace A) : Prop :=
-{   L_FORM : t = trace_app (trace_fin (l1 ++ [x] ++ l2 ++ [y])) rest;
-    R_FORM : t' = trace_app (trace_fin (l1 ++ [y] ++ l2 ++ [x])) rest;
+Record lsc A (a b l1 l2 : list A) x y : Prop :=
+{   L1_EQ : a = l1 ++ [x] ++ l2 ++ [y];
+    L2_EQ : b = l1 ++ [y] ++ l2 ++ [x];
 }.
 
-Lemma swapped_sym l1 l2 rest x y t t'
-    (SWAPPED : t_constructive_gen l1 l2 rest x y t t') :
-    t_constructive_gen l1 l2 rest y x t' t.
-Proof using.
-    destruct SWAPPED; subst t t'.
+Definition ls A a b m n :=
+    exists l1 l2 x y,
+        ⟪ STRUCT : lsc A a b l1 l2 x y ⟫ /\
+        ⟪ L1_LEN : length l1 = m ⟫ /\
+        ⟪ L2_LEN : length l1 + 1 + length l2 = n ⟫.
+
+Definition trace_swapped A t t' m n : Prop :=
+    exists l l' rest,
+        ⟪ SWAP : ls A l l' m n ⟫ /\
+        ⟪ STRUCT1 : t = trace_app (trace_fin l) rest ⟫ /\
+        ⟪ STRUCT2 : t' = trace_app (trace_fin l') rest ⟫.
+
+Global Hint Unfold ls trace_swapped : unfolderDb.
+
+Section ListsSwappedConstr.
+
+Variable A : Type.
+Variable a b l1 l2 : list A.
+Variable x y : A.
+Hypothesis SWAPPED : lsc A a b l1 l2 x y.
+
+Lemma lsc_sym : lsc A b a l1 l2 y x.
+Proof using SWAPPED.
+    destruct SWAPPED; subst a b.
     constructor; ins.
 Qed.
 
-Lemma swapped_len l1 l2 rest x y t t'
-    (SWAPPED : t_constructive_gen l1 l2 rest x y t t') :
-    trace_length t' = trace_length t.
-Proof using.
-    destruct SWAPPED; subst t t'.
-    rewrite !trace_length_app. simpl.
-    change (y :: l2 ++ [x]) with ([y] ++ l2 ++ [x]).
-    change (x :: l2 ++ [y]) with ([x] ++ l2 ++ [y]).
-    now do 6 rewrite length_app.
+Lemma lsc_len_eq : length b = length a.
+Proof using SWAPPED.
+    destruct SWAPPED; subst a b.
+    now autorewrite with calc_length.
 Qed.
 
-Lemma swapped_l2_len l1 l2 rest x y t t'
-    (SWAPPED : t_constructive_gen l1 l2 rest x y t t') :
-    NOmega.lt_nat_l (length l1 + 1 + length l2) (trace_length t').
-Proof using.
-    destruct SWAPPED; subst t'.
-    rewrite trace_length_app; simpl.
-    change (y :: l2 ++ [x]) with ([y] ++ l2 ++ [x]).
-    do 3 rewrite length_app.
-    destruct trace_length; try easy.
-    simpl. lia.
+Lemma lsc_len : length a = length l1 + 1 + length l2 + 1.
+Proof using SWAPPED.
+    destruct SWAPPED; subst a b.
+    autorewrite with calc_length; lia.
 Qed.
 
-Lemma swapped_l1_len l1 l2 rest x y t t'
-    (SWAPPED : t_constructive_gen l1 l2 rest x y t t') :
-    NOmega.lt_nat_l (length l1) (trace_length t').
-Proof using.
-    eapply NOmega.lt_lt_nat.
-    2: eapply swapped_l2_len; exact SWAPPED.
-    lia.
+Hint Rewrite lsc_len_eq lsc_len : lsc.
+
+Lemma lsc_len_1 :
+    length l1 < length b.
+Proof using SWAPPED.
+    autorewrite with calc_length lsc; lia.
 Qed.
 
-Lemma swapped_nth_1 l1 l2 rest x y t t' n d
-    (SWAPPED : t_constructive_gen l1 l2 rest x y t t')
+Lemma lsc_len_2 :
+    length l1 + 1 + length l2 < length b.
+Proof using SWAPPED.
+    autorewrite with calc_length lsc; lia.
+Qed.
+
+Lemma lsc_nth_1 n d
     (LT : n < length l1) :
-    trace_nth n t' d = trace_nth n t d.
-Proof using.
-    destruct SWAPPED; subst t t'.
-    rewrite !trace_nth_app. simpl.
-    rewrite !length_app.
-    do 2 destruct (excluded_middle_informative _); try lia.
-    rewrite !nth_app.
-    destruct (Compare_dec.le_lt_dec _ _); auto.
-    exfalso; lia.
+    nth n b d = nth n a d.
+Proof using SWAPPED.
+    destruct SWAPPED; subst a b.
+    now rewrite !app_nth1 by auto.
 Qed.
 
-Lemma swapped_nth_2 l1 l2 rest x y t t' n d
-    (SWAPPED : t_constructive_gen l1 l2 rest x y t t')
+Lemma lsc_nth_2 n d
     (LT : length l1 < n)
-    (LT' : n < length l1 + 1 + length l2):
-    trace_nth n t' d = trace_nth n t d.
-Proof using.
-    destruct SWAPPED; subst t t'.
-    rewrite !trace_nth_app. simpl.
-    do 2 (rewrite !length_app; simpl).
-    destruct (excluded_middle_informative _); try lia.
-    rewrite !nth_app.
-    destruct (Compare_dec.le_lt_dec _ _); auto.
-    change (y :: l2 ++ [x]) with ([y] ++ l2 ++ [x]).
-    change (x :: l2 ++ [y]) with ([x] ++ l2 ++ [y]).
-    rewrite !nth_app.
-    destruct (Compare_dec.le_lt_dec _ _); try solve [simpl in *; lia].
-    destruct (Compare_dec.le_lt_dec _ _); try solve [simpl in *; lia].
-    done.
+    (LT' : n < length l1 + 1 + length l2) :
+    nth n b d = nth n a d.
+Proof using SWAPPED.
+    destruct SWAPPED; subst a b.
+    rewrite !app_assoc with (l := l1).
+    rewrite !app_nth2 with (l := l1 ++ [_]).
+    all: autorewrite with calc_length; try lia.
+    now rewrite !app_nth1 by lia.
 Qed.
 
-Lemma swapped_nth_3 l1 l2 rest x y t t' n d
-    (SWAPPED : t_constructive_gen l1 l2 rest x y t t')
-    (LT : length l1 + 1 + length l2 < n):
-    trace_nth n t' d = trace_nth n t d.
-Proof using.
-    destruct SWAPPED; subst t t'.
-    rewrite !trace_nth_app. simpl.
-    do 2 (rewrite !length_app; simpl).
-    now destruct (excluded_middle_informative _); try lia.
-Qed.
-
-Lemma swapped_nth_x l1 l2 rest x y t t' d
-    (SWAPPED : t_constructive_gen l1 l2 rest x y t t') :
-    trace_nth (length l1) t' d = y.
-Proof using.
-    destruct SWAPPED; subst t t'.
-    rewrite !trace_nth_app. simpl.
-    do 2 (rewrite !length_app; simpl).
-    destruct (excluded_middle_informative _); try lia.
-    rewrite nth_app.
-    destruct (Compare_dec.le_lt_dec _ _); try lia.
+Lemma lsc_nth_y d :
+    nth (length l1) b d = y.
+Proof using SWAPPED.
+    destruct SWAPPED; subst a b.
+    rewrite app_nth2 by lia.
     now rewrite PeanoNat.Nat.sub_diag.
 Qed.
 
-Lemma swapped_nth_y l1 l2 rest x y t t' d
-    (SWAPPED : t_constructive_gen l1 l2 rest x y t t') :
-    trace_nth (length l1 + 1 + length l2) t' d = x.
-Proof using.
-    destruct SWAPPED; subst t t'.
-    rewrite !trace_nth_app. simpl.
-    do 2 (rewrite !length_app; simpl).
-    destruct (excluded_middle_informative _); try lia.
-    rewrite nth_app.
-    destruct (Compare_dec.le_lt_dec _ _); try lia.
-    change (y :: l2 ++ [x]) with ([y] ++ l2 ++ [x]).
-    rewrite nth_app.
-    destruct (Compare_dec.le_lt_dec _ _); try solve [simpl in *; lia].
-    rewrite nth_app.
-    destruct (Compare_dec.le_lt_dec _ _); try solve [simpl in *; lia].
-    simpl.
-    arewrite (length l1 + 1 + length l2 - length l1 - 1 - length l2 = 0) by lia.
+Lemma lsc_nth_x d :
+    nth (length l1 + 1 + length l2) b d = x.
+Proof using SWAPPED.
+    destruct SWAPPED; subst a b.
+    rewrite !app_assoc.
+    rewrite <- app_assoc with (l := l1) (n := l2).
+    rewrite app_nth2.
+    all: autorewrite with calc_length; try lia.
+    now rewrite PeanoNat.Nat.add_assoc, PeanoNat.Nat.sub_diag.
 Qed.
 
-Lemma swapped_nth l1 l2 rest x y t t' n d
-    (SWAPPED : t_constructive_gen l1 l2 rest x y t t')
+Lemma lsc_nth n d
     (NEQ1 : n <> length l1)
     (NEQ2 : n <> length l1 + 1 + length l2) :
-    trace_nth n t' d = trace_nth n t d.
-Proof using.
-    destruct (NPeano.Nat.lt_total n (length l1)) as [LT | [EQ | GT]].
-    all: destruct (NPeano.Nat.lt_total n (length l1 + 1 + length l2)) as [LT' | [EQ' | GT']].
-    all: try lia.
-    all: eauto using swapped_nth_1, swapped_nth_2, swapped_nth_3.
+    nth n b d = nth n a d.
+Proof using SWAPPED.
+    destruct (NPeano.Nat.lt_total n (length l1)).
+    all: destruct (NPeano.Nat.lt_total n (length l1 + 1 + length l2)).
+    all: desf; try lia.
+    all: eauto using lsc_nth_1, lsc_nth_2.
+    rewrite !nth_overflow; auto.
+    all: autorewrite with lsc; lia.
 Qed.
 
-Lemma all_finite (l : list A) :
-    trace_finite (trace_fin l).
-Proof using.
-    unfold trace_finite. eauto.
+Lemma lsc_in : (fun x => In x a) ≡₁ (fun x => In x b).
+Proof using SWAPPED.
+    destruct SWAPPED; subst a b.
+    unfolder. splits.
+    all: intros; rewrite !in_app_iff in *.
+    all: desf; eauto.
 Qed.
 
-Lemma swapped_same_elems_sub l1 l2 rest x y t t'
-    (SWAPPED : t_constructive_gen l1 l2 rest x y t t') :
-    trace_elems t ≡₁ trace_elems t'.
-Proof using.
-    destruct SWAPPED; subst t t'.
-    rewrite !trace_elems_app.
-    do 2 destruct excluded_middle_informative.
-    all: try solve [exfalso; eauto using all_finite].
-    simpl. unfolder. splits; intros e HIN.
-    all: do 2 (rewrite in_app_iff in *; simpl in *).
-    all: desf; tauto.
+Lemma lsc_impl_ls : ls A a b (length l1) (length l1 + 1 + length l2).
+Proof using SWAPPED.
+    destruct SWAPPED; subst a b.
+    unfolder. repeat econstructor.
 Qed.
 
-Definition trace_swapped t t' n m : Prop :=
-    exists l1 l2 rest x y,
-        ⟪ L1_LEN : length l1 = n ⟫ /\
-        ⟪ L2_LEN : length l2 = m ⟫ /\
-        ⟪ STRUCT : t_constructive_gen l1 l2 rest x y t t' ⟫.
+End ListsSwappedConstr.
 
+Global Hint Resolve lsc_sym lsc_len_eq lsc_len lsc_nth_1 lsc_nth_2 lsc_nth
+    lsc_impl_ls lsc_in : lsc.
 
+Section ListsSwapped.
+
+Variable A : Type.
+Variable a b : list A.
+Variable m n : nat.
+Hypothesis SWAPPED : ls A a b m n.
+
+Lemma ls_sym : ls A b a m n.
+Proof using SWAPPED.
+    destruct SWAPPED; desc; subst n m.
+    repeat econstructor; apply STRUCT.
+Qed.
+
+Lemma ls_len_eq : length b = length a.
+Proof using SWAPPED.
+    destruct SWAPPED; desc; subst n m.
+    eauto with lsc.
+Qed.
+
+Lemma ls_len : length a = n + 1.
+Proof using SWAPPED.
+    destruct SWAPPED; desc; subst n m.
+    eauto with lsc.
+Qed.
+
+Lemma ls_lt_m : m < n.
+Proof using SWAPPED.
+    destruct SWAPPED; desc; subst n m.
+    lia.
+Qed.
+
+Lemma ls_lt_n : n < length a.
+Proof using SWAPPED.
+    rewrite ls_len; lia.
+Qed.
+
+Lemma ls_nth_1 N d
+    (LT : N < m) :
+    nth N b d = nth N a d.
+Proof using SWAPPED.
+    destruct SWAPPED; desc; subst n m.
+    eauto with lsc.
+Qed.
+
+Lemma ls_nth_2 N d
+    (LT : m < N)
+    (LT' : N < n) :
+    nth N b d = nth N a d.
+Proof using SWAPPED.
+    destruct SWAPPED; desc; subst n m.
+    eauto with lsc.
+Qed.
+
+Lemma ls_nth_y d :
+    nth n b d = nth m a d.
+Proof using SWAPPED.
+    destruct SWAPPED; desc; subst n m.
+    now erewrite lsc_nth_x, lsc_nth_y by eauto with lsc.
+Qed.
+
+Lemma ls_nth_x d :
+    nth m b d = nth n a d.
+Proof using SWAPPED.
+    destruct SWAPPED; desc; subst n m.
+    now erewrite lsc_nth_x, lsc_nth_y by eauto with lsc.
+Qed.
+
+Lemma ls_nth N d
+    (NEQ1 : N <> m)
+    (NEQ2 : N <> n) :
+    nth N b d = nth N a d.
+Proof using SWAPPED.
+    destruct SWAPPED; desc; subst n m.
+    eauto with lsc.
+Qed.
+
+Lemma ls_in : (fun x => In x a) ≡₁ (fun x => In x b).
+Proof using SWAPPED.
+    destruct SWAPPED; desc.
+    eauto with lsc.
+Qed.
+
+End ListsSwapped.
+
+Global Hint Resolve ls_sym ls_len ls_len_eq ls_nth_1 ls_nth_2 ls_nth
+    ls_nth_x ls_nth_y ls_lt_m ls_lt_n ls_in : ls.
+
+Section TracesSwapped.
+
+Variable A : Type.
+Variable t t' : trace A.
+Variable m n : nat.
+Variable SWAPPED : trace_swapped A t t' m n.
+
+Lemma trace_swapped_sym : trace_swapped A t' t m n.
+Proof using SWAPPED.
+    destruct SWAPPED as (l & l' & SWAPPED'); desc; subst t t'.
+    exists l'; exists l; exists rest.
+    splits; eauto with ls.
+Qed.
+
+Lemma trace_swapped_len : trace_length t' = trace_length t.
+Proof using SWAPPED.
+    destruct SWAPPED; desc; subst t t'.
+    destruct rest; simpl; try easy.
+    autorewrite with calc_length; do 2 f_equal.
+    eauto with ls.
+Qed.
+
+Lemma trace_swapped_lt_m : m < n.
+Proof using SWAPPED.
+    destruct SWAPPED; desc; subst t t'.
+    eauto with ls.
+Qed.
+
+Lemma trace_swapped_lt_n : NOmega.lt_nat_l n (trace_length t).
+Proof using SWAPPED.
+    destruct SWAPPED; desc; subst t t'.
+    rewrite trace_length_app.
+    destruct (trace_length rest); simpl; try easy.
+    eauto using PeanoNat.Nat.lt_lt_add_r with ls.
+Qed.
+
+(* TODO: useful for hahn? *)
+Lemma trace_nth_app1 (a b : trace A) N d
+    (LT : NOmega.lt_nat_l N (trace_length a)) :
+    trace_nth N (trace_app a b) d = trace_nth N a d.
+Proof using.
+    rewrite trace_nth_app.
+    destruct excluded_middle_informative; auto.
+    now exfalso.
+Qed.
+
+Lemma trace_nth_app2 (a : list A) (b : trace A) N d
+    (LT : length a <= N) :
+    trace_nth N (trace_app (trace_fin a) b) d = trace_nth (N - length a) b d.
+Proof using.
+    rewrite trace_nth_app.
+    destruct excluded_middle_informative; simpl in *; auto.
+    lia.
+Qed.
+
+Lemma trace_swapped_nth_1 N d
+    (LT : N < m) :
+    trace_nth N t' d = trace_nth N t d.
+Proof using SWAPPED.
+    assert (LT' : m < n) by apply trace_swapped_lt_m.
+    destruct SWAPPED; desc; subst t t'.
+    rewrite !trace_nth_app1; simpl; eauto with ls.
+    all: erewrite ls_len; eauto with ls; lia.
+Qed.
+
+Lemma trace_swapped_nth_2 N d
+    (LT : m < N)
+    (LT' : N < n) :
+    trace_nth N t' d = trace_nth N t d.
+Proof using SWAPPED.
+    destruct SWAPPED; desc; subst t t'.
+    rewrite !trace_nth_app1; simpl; eauto with ls.
+    all: erewrite ls_len; eauto with ls; lia.
+Qed.
+
+Lemma trace_swapped_nth_3 N d
+    (LT : n < N) :
+    trace_nth N t' d = trace_nth N t d.
+Proof using SWAPPED.
+    destruct SWAPPED; desc; subst t t'.
+    rewrite !trace_nth_app2; simpl.
+    all: erewrite !ls_len; eauto with ls; lia.
+Qed.
+
+Lemma trace_swapped_nth_y d :
+    trace_nth n t' d = trace_nth m t d.
+Proof using SWAPPED.
+    assert (LT' : m < n) by apply trace_swapped_lt_m.
+    destruct SWAPPED; desc; subst t t'.
+    rewrite !trace_nth_app1; simpl; eauto with ls.
+    erewrite ls_len; eauto with ls; lia.
+Qed.
+
+Lemma trace_swapped_nth_x d :
+    trace_nth m t' d = trace_nth n t d.
+Proof using SWAPPED.
+    assert (LT' : m < n) by apply trace_swapped_lt_m.
+    destruct SWAPPED; desc; subst t t'.
+    rewrite !trace_nth_app1; simpl; eauto with ls.
+    erewrite ls_len; eauto with ls; lia.
+Qed.
+
+Lemma trace_swapped_nth N d
+    (NEQ1 : N <> m)
+    (NEQ2 : N <> n) :
+    trace_nth N t d = trace_nth N t' d.
+Proof using SWAPPED.
+    destruct SWAPPED; desc; subst t t'.
+    destruct (PeanoNat.Nat.lt_ge_cases N (n + 1)).
+    { rewrite !trace_nth_app1; simpl; eauto with ls.
+      all: erewrite ls_len; eauto with ls; lia. }
+    rewrite !trace_nth_app2.
+    all: erewrite !ls_len; eauto with ls.
+Qed.
+
+Lemma trace_swapped_elems : trace_elems t ≡₁ trace_elems t'.
+Proof using SWAPPED.
+    destruct SWAPPED; desc; subst t t'.
+    rewrite !trace_elems_app. simpl.
+    rewrite ls_in by eauto.
+    assert (FIN : forall (l : list A), trace_finite (trace_fin l)) by (intros; red; eauto).
+    do 2 destruct excluded_middle_informative; try solve [exfalso; eauto].
+    done.
+Qed.
+
+End TracesSwapped.
+
+Global Hint Resolve trace_swapped_sym trace_swapped_len trace_swapped_lt_m
+    trace_swapped_lt_n trace_swapped_nth_1 trace_swapped_nth_2 trace_swapped_nth_3
+    trace_swapped_nth_x trace_swapped_nth_y trace_swapped_nth trace_swapped_elems
+     : trace_swap.
